Hoare.v
@@ -1,0 +1,74 @@
+(* Adapted with minimal modifications from Hoare Logic, Part I
+   (Hoare) of Programming Language Foundations:
+   https://softwarefoundations.cis.upenn.edu/plf-current/Hoare.html *)
+
+From Coq Require Import Strings.String Program.Equality.
+From LongDivision Require Import Maps Imp.
+
+(* Core definitions *)
+
+Definition Assertion := state -> Prop.
+
+Definition assert_implies (P Q : Assertion) : Prop :=
+  forall st, P st -> Q st.
+
+Notation "P '->>' Q" := (assert_implies P Q) (at level 80) :
+  hoare_spec_scope.
+
+Open Scope hoare_spec_scope.
+
+Definition hoare_triple (P : Assertion) (c : com) (Q : Assertion)
+  : Prop := forall st st', P st -> st =[ c ]=> st' -> Q st'.
+
+Notation "'{{' P '}}' c '{{' Q '}}'" := (hoare_triple P c Q)
+  (at level 90, c at next level) : hoare_spec_scope.
+
+(* Proof rules *)
+
+Ltac inv H := inversion H; subst; clear H.
+
+Theorem hoare_floyd : forall P x a,
+  {{ P }} x ::= a {{ fun st => exists st',
+  (forall y, x <> y -> st y = st' y) /\
+  st x = aeval st' a /\
+  P st' }}.
+Proof with auto.
+  unfold hoare_triple; intros; inv H0; unfold t_update.
+  exists st; repeat split...
+  - intros; destruct (string_dec x y)...
+    contradiction H0.
+  - destruct (string_dec x x)...
+    now contradiction n.
+Qed.
+
+Theorem hoare_consequence : forall P P' Q Q' c,
+  {{ P' }} c {{ Q' }} ->
+  P ->> P' ->
+  Q' ->> Q ->
+  {{ P }} c {{ Q }}.
+Proof. unfold hoare_triple; eauto. Qed.
+
+Theorem hoare_skip : forall P, {{ P }} SKIP {{ P }}.
+Proof. unfold hoare_triple; intros; now inv H0. Qed.
+
+Theorem hoare_seq : forall P Q R c1 c2,
+  {{ P }} c1 {{ Q }} ->
+  {{ Q }} c2 {{ R }} ->
+  {{ P }} c1 ;; c2 {{ R }}.
+Proof. unfold hoare_triple; intros; inv H2; eauto. Qed.
+
+Theorem hoare_if : forall P Q b c1 c2,
+  {{ fun st => P st /\ beval st b = true }} c1 {{ Q }} ->
+  {{ fun st => P st /\ beval st b = false }} c2 {{ Q }} ->
+  {{ P }} TEST b THEN c1 ELSE c2 FI {{ Q }}.
+Proof. unfold hoare_triple; intros; inv H2; eauto. Qed.
+
+Theorem hoare_while : forall P b c',
+  {{ fun st => P st /\ beval st b = true }} c' {{ P }} ->
+  {{ P }} WHILE b DO c' END {{ fun st => P st /\
+  beval st b = false }}.
+Proof.
+  unfold hoare_triple; intros; dependent induction H1; eauto.
+Qed.
+
+Close Scope hoare_spec_scope.
